18 sep

coq/delayed.v
@@ -9,18 +9,24 @@ Definition delayed_val {A : Type} (x: A) := Delayed (inl x).
 Definition delayed_del {A : Type} (x: delayed A) := Delayed (inr x).
 
 CoFixpoint map {A B: Type} (f : A -> B) (x : delayed A) : delayed B :=
-  match state x with
-  | inl a => delayed_val (f a)
-  | inr x' => delayed_del (map f x')
-  end.
+{|
+  state :=
+    match state x with
+    | inl a => inl (f a)
+    | inr x' => inr (map f x')
+    end
+|}.
 
-Definition pure {A: Type} (v: A) := delayed_val v.
+Definition pure {A : Type} (v: A) := delayed_val v.
 
-CoFixpoint bind {A B: Type} (x : delayed A) (f : A -> delayed B) : delayed B :=
-  match state x with
-  | inl a => f a
-  | inr x' => delayed_del (bind x' f)
-  end.
+CoFixpoint bind {A B : Type} (x : delayed A) (f : A -> delayed B) : delayed B :=
+{|
+  state :=
+    match state x with
+    | inl a => state (f a)
+    | inr x' => inr (bind x' f)
+    end
+|}.
 
 CoFixpoint constDelayed {A: Type} (x: A) (t: nat) : delayed A :=
   match t with
@@ -35,57 +41,60 @@ Proof.
   now intros A [] []; cbn; intros [].
 Qed.
 
-Inductive EqDelayed {A: Type} : delayed A -> delayed A -> Prop :=
-| EqRes : forall x: A, EqDelayed (delayed_val x) (delayed_val x)
-| EqDel : forall x y : delayed A, EqDelayed x y -> EqDelayed (delayed_del x) (delayed_del y).
+Inductive SimF {A: Type} (x y : delayed A) (R: delayed A -> delayed A -> Prop) : Prop :=
+| SimF_val : forall (v : A), state x = inl v -> state y = inl v ->
+   SimF x y R
+| SimF_del : forall (x' y' : delayed A), state x = inr x' -> state y = inr y' ->
+   R x' y' -> SimF x y R.
 
-CoInductive Eq_delayed {A: Type} : delayed A -> delayed A -> Prop :=
-  state_eq : forall x y : delayed A,
-    (exists v: A, state x = inl v /\ state y = inl v) \/
-    (exists x' y': delayed A, Eq_delayed x' y' /\ state x = inr x' /\ state y = inr y')
-     -> Eq_delayed x y.
+CoInductive Sim {A: Type} (x y: delayed A) : Prop := {
+  out : SimF x y Sim
+}.
 
-Lemma map_id (A: Type) (x: delayed A) : Eq_delayed (map id x) x.
+Axiom delayed_eq : forall (A: Type) (x y : delayed A), Sim x y -> x = y. 
+
+Lemma map_id (A: Type) (x: delayed A) : (map id x) = x.
 Proof.
-  revert A x. cofix CH. destruct x as [[v | d]].
-  - constructor. left. exists v. cbn. split; reflexivity.
-  - constructor. right. cbn. exists (map id d), d. split; cycle 1. split; auto.
-    apply CH.
+  apply delayed_eq. revert A x. cofix CH. destruct x as [[v | d]].
+  - constructor. apply SimF_val with (v0 := v); auto.
+  - constructor. apply SimF_del with (x' := (map id d)) (y' :=  d); auto.
 Qed.
 
 Definition dot {A B C: Type} (f : B -> C) (g: A -> B) (x: A) := f (g x).
 Notation "f (.) g" := (dot f g) (at level 75). 
 
 Lemma map_comp (A B C: Type) (f : B -> C) (g: A -> B) (x: delayed A) : 
-  Eq_delayed (map (f (.) g) x) (map f (map g x)).
+  (map (f (.) g) x) = (map f (map g x)).
 Proof.
-  revert A B C f g x. cofix CH. destruct x as [[v | d]].
-  - constructor. left. exists (f (g v)). unfold dot. cbn. split; auto.
-  - constructor. right. cbn. exists (map (f (.) g) d), (map f (map g d)).
-    split; cycle 1. split; auto. apply CH.
+  apply delayed_eq. revert A B C f g x. cofix CH. destruct x as [[v | d]].
+  - constructor. apply SimF_val with (v0 := (f (g v))); auto.
+  - constructor. apply SimF_del with (x' := (map (f (.) g) d)) (y' := (map f (map g d))); auto. 
 Qed.
 
 Lemma left_id_bind (A B : Type) (f: A -> delayed B) (x: A) : 
-  Eq_delayed (bind (pure x) f) (f x).
+  (bind (pure x) f) = (f x).
 Proof.
-  unfold pure, delayed_val. destruct (bind {| state := inl x |} f) eqn:e.
-  constructor. destruct state0.
+  apply delayed_eq.
+  destruct (f x) as [[b | d]] eqn: Heq.
+  - now econstructor; cbn; [rewrite Heq |].
+  - econstructor 2; cbn; [now rewrite Heq | easy |].
+    apply Sim_refl.
+Qed.
 Abort.
 
 Lemma right_id_bind (A B : Type) (x: delayed A) : 
-  Eq_delayed (bind x pure) x.
+  (bind x pure) = x.
 Proof.
-  revert A x. cofix CH. destruct x as [[v | d]].
-  - constructor. left. exists v. cbn. split; reflexivity.
-  - constructor. right. cbn. exists (bind d pure), d. split; cycle 1. split; auto.
-    apply CH.
+  apply delayed_eq. revert A x. cofix CH. destruct x as [[v | d]].
+  - constructor. apply SimF_val with (v0 := v); auto.
+  - constructor. apply SimF_del with (x' := (bind d pure)) (y' :=  d); auto.
 Qed.
 
 Lemma bind_comp (A B C: Type) (f : B -> delayed C) (g: A -> delayed B) (x: delayed A) : 
-  Eq_delayed (bind (bind x g) f) (bind x (fun y => bind (g y) f)).
+  (bind (bind x g) f) = (bind x (fun y => bind (g y) f)).
 Proof.
-  revert A B C f g x. cofix CH. destruct x as [[v | d]].
-  - constructor. left. exists (f (g v)). unfold dot. cbn. split; auto.
+  apply delayed_eq. revert A B C f g x. cofix CH. destruct x as [[v | d]].
+  - constructor. apply SimF_val with (v0 := (bind (g v) f)). exists (f (g v)). unfold dot. cbn. split; auto.
   - constructor. right. cbn. exists (map (f (.) g) d), (map f (map g d)).
     split; cycle 1. split; auto. apply CH.
 Qed.
