coq/FreeGroup.v
@@ -1,0 +1,108 @@
+Require Import Coq.Program.Equality.
+Require Import Coq.Bool.Bool.
+Require Import Coq.Lists.List.
+Import ListNotations.
+
+Class Group (A : Type) := GroupDef {
+  zero      : A;
+  op        : A -> A -> A;
+  inv       : A -> A;
+  eqf       : A -> A -> bool;
+  left_id   : forall x: A, op zero x = x;
+  right_id  : forall x: A, op x zero = x;
+  left_inv  : forall x: A, op (inv x) x = zero;
+  right_inv : forall x: A, op x (inv x) = zero;
+  op_assoc  : forall x y z: A, op (op x y) z = op x (op y z);
+  eqf_eq    : forall x y, reflect (x = y) (eqf x y)
+}.
+
+Print reflect.
+
+Lemma eqf_refl {A: Type} `{Group A} (x : A) : eqf x x = true.
+Proof.
+  destruct (eqf_eq x x); auto.
+Qed.
+
+Definition eqf_false {A: Type} `{Group A} {x y: A} : eqf x y = false -> x <> y.
+Proof.
+  intros H0 H1. subst. rewrite eqf_refl in H0. discriminate.
+Defined.
+
+Notation "a @ b" := (op a b) (at level 50).
+Notation "c ^" := (inv c) (at level 40).
+
+Definition sub {A: Type} `{Group A} (x y: A) := op x (inv y).
+
+Definition CanonFreeGroup (A: Type) `{Group A} := list (bool*A).
+
+Inductive NonEmptyFreeGroup (A: Type) `{Group A} :=
+| Singl  : bool -> A -> NonEmptyFreeGroup A
+| Switch : forall x: A, eqf zero x = false -> NonEmptyFreeGroup A -> NonEmptyFreeGroup A
+| Stay   : A -> NonEmptyFreeGroup A -> NonEmptyFreeGroup A.
+
+Arguments Switch {A H}.
+Arguments Stay {A H}.
+Arguments Singl {A H}.
+
+Definition FreeGroup (A: Type) `{Group A} := option (NonEmptyFreeGroup A).
+
+Fixpoint to_uniq' {A: Type} `{Group A} (b : bool) (v: A) (x: CanonFreeGroup A) : NonEmptyFreeGroup A :=
+match x with 
+| []             => Singl b v
+| (b', v') :: x' => if eqb b b' 
+                      then Stay (sub v v') (to_uniq' b' v' x')
+                      else match eqf zero (sub v v') as i return (eqf zero (sub v v') = i) -> NonEmptyFreeGroup A with
+                           | false => fun e => Switch (sub v v') e (to_uniq' b' v' x')
+                           | true  => fun _ => (Singl b v) (* invalid *)
+                           end eq_refl
+end.
+
+Definition to_uniq {A: Type} `{Group A} (x: CanonFreeGroup A) : FreeGroup A :=
+match x with
+| [] => None
+| (b, v) :: x' => Some (to_uniq' b v x')
+end.
+
+Fixpoint to_canon' {A: Type} `{Group A} (x: NonEmptyFreeGroup A) : CanonFreeGroup A :=
+  match x with 
+  | Singl b v   => [(b, v)]
+  | Stay v x'   => match to_canon' x' with
+                   | [] => [(true, v)] (* should not be there *)
+                   | (b, v') :: y => (b, (v @ v')) :: (b, v') :: y
+                   end
+  | Switch v _ x' => match to_canon' x' with
+                               | [] => [(true, v)] (* should not be there *)
+                               | (b, v') :: y => (negb b, (v @ v')) :: (b, v') :: y
+                               end
+  end.
+
+Definition to_canon {A: Type} `{Group A} (x: FreeGroup A) : CanonFreeGroup A :=
+  match x with
+  | None => []
+  | Some x' => to_canon' x'
+  end.
+
+Lemma op_sub {A: Type} `{Group A} (x y : A) : op (sub x y) y = x.
+Proof.
+  unfold sub. rewrite op_assoc. rewrite left_inv. rewrite right_id. auto.
+Qed.
+
+Lemma sub_op {A: Type} `{Group A} (x y : A) : sub (op x y) y = x.
+Proof.
+  unfold sub. rewrite op_assoc. rewrite right_inv. rewrite right_id. auto.
+Qed.
+
+Print reflect.
+
+Theorem free_group_epi_cannon {A: Type} `{Group A} (x: FreeGroup A) : 
+  to_uniq (to_canon x) = x.
+Proof.
+  destruct x as [x |].
+  - induction x; auto.
+    + cbn in *. destruct x0.
+      * cbn. f_equal. rewrite eqb_negb1, sub_op. dependent destruction x1.
+
+
+
+
+
